CBOR generic data model

src/cbor/CBOR.Spec.Type.fsti
@@ -40,11 +40,142 @@ noextract
 let simple_value : eqtype =
   (x: U8.t { simple_value_wf x == true } )
 
-(* Raw data items, disregarding ordering of map entries *)
+(* The generic data model *)
+
+let u0 = CBOR.Spec.FiniteMap.UniverseToken u#0
 
 noextract
 noeq
-type raw_data_item
+type cbor_case (t: Type u#a) : Type u#(max a 1) =
+  | CSimple: (v: simple_value) -> cbor_case t
+  | CInt64: (typ: major_type_uint64_or_neg_int64) -> (v: U64.t) -> cbor_case t
+  | CString: (typ: major_type_byte_string_or_text_string) -> (v: Seq.seq U8.t { FStar.UInt.fits (Seq.length v) U64.n }) -> cbor_case t // Section 3.1: "a string containing an invalid UTF-8 sequence is well-formed but invalid", so we don't care about UTF-8 specifics here.
+  | CArray: (v: list t { FStar.UInt.fits (List.Tot.length v) U64.n }) -> cbor_case t
+  | CMap: (c: CBOR.Spec.FiniteMap.fmap t t u0 { FStar.UInt.fits (CBOR.Spec.FiniteMap.length c) U64.n }) -> cbor_case t
+  | CTagged: (tag: U64.t) -> (v: t) -> cbor_case t
+
+let rec list_eq
+  (#t: Type)
+  (eq: CBOR.Spec.FiniteMap.eq_test t)
+  (l1 l2: list t)
+: Tot (CBOR.Spec.FiniteMap.eq_elem_test_codom l1 l2)
+  (decreases l1)
+= match l1, l2 with
+  | [], [] -> true
+  | x1 :: l1', x2 :: l2' -> eq x1 x2 && list_eq eq l1' l2'
+  | _ -> false
+
+let rec seq_eq
+  (#t: Type)
+  (eq: CBOR.Spec.FiniteMap.eq_test t)
+  (l1 l2: Seq.seq t)
+: Tot (CBOR.Spec.FiniteMap.eq_elem_test_codom l1 l2)
+  (decreases (Seq.length l1))
+= if Seq.length l1 = 0
+  then
+    if Seq.length l2 = 0
+    then begin
+      assert (l1 `Seq.equal` l2);
+      true
+    end
+    else false
+  else if Seq.length l2 = 0
+  then false
+  else begin
+    Seq.cons_head_tail l1;
+    Seq.cons_head_tail l2;
+    eq (Seq.head l1) (Seq.head l2) && seq_eq eq (Seq.tail l1) (Seq.tail l2)
+  end
+
+let cbor_case_eq
+  (#t: Type)
+  (eq: CBOR.Spec.FiniteMap.eq_test t)
+: Tot (CBOR.Spec.FiniteMap.eq_test (cbor_case t))
+= fun c1 c2 -> match c1, c2 with
+  | CSimple v1, CSimple v2 -> v1 = v2
+  | CInt64 t1 v1, CInt64 t2 v2 -> t1 = t2 && v1 = v2
+  | CString t1 s1, CString t2 s2 -> t1 = t2 && seq_eq (fun x y -> x = y) s1 s2
+  | CArray l1, CArray l2 -> list_eq eq l1 l2
+  | CMap l1, CMap l2 -> CBOR.Spec.FiniteMap.fmap_eq l1 l2
+  | CTagged tag1 x1, CTagged tag2 x2 -> tag1 = tag2 && eq x1 x2
+  | _ -> false
+
+let rec list_bound
+  (#t: Type)
+  (bound: t -> Tot nat)
+  (l: list t)
+: Tot nat
+= match l with
+  | [] -> 0
+  | a :: q ->
+    let ba = bound a in
+    let bq = list_bound bound q in
+    if ba >= bq then ba else bq
+
+let fmap_bound_op
+  (#t: Type)
+  (s: CBOR.Spec.FiniteMap.fmap t t u0)
+  (bound: t -> Tot nat)
+  (accu: nat)
+  (x: t)
+: Tot nat
+= let bx = bound x in
+  let accu1 = if bx > accu then bx else accu in
+  let bw = match CBOR.Spec.FiniteMap.get x s with
+  | None -> 0
+  | Some w -> bound w
+  in
+  if bw > accu1 then bw else accu1
+
+let fmap_bound
+  (#t: Type)
+  (bound: t -> Tot nat)
+  (s: CBOR.Spec.FiniteMap.fmap t t u0)
+: Tot nat
+= CBOR.Spec.FiniteMap.fold (fmap_bound_op s bound) 0 s
+
+let cbor_case_bound
+  (#t: Type)
+  (bound: t -> nat)
+  (x: cbor_case t)
+: Tot nat
+= match x with
+  | CArray l -> 1 + list_bound bound l
+  | CMap l -> 1 + fmap_bound bound l
+  | CTagged _ x -> 1 + bound x
+  | _ -> 0
+
+[@@erasable] noeq type empty_t : Type u#a =
+
+noextract [@@noextract_to "krml"]
+let empty_elim (#t: Type u#b) (x: empty_t u#a) : Tot t =
+  match empty_t with
+
+let rec cbor1 (b: nat) : Tot (Type u#1)
+  (decreases (b + b + 1))
+= cbor_case (cbor2 b)
+
+and cbor2 (b: nat) : Tot (Type u#1)
+  (decreases (b + b))
+= (if b = 0 then empty_t else cbor1 (b - 1))
+
+let rec cbor1_bound (b: nat) : Tot (cbor1 b -> nat) (decreases (b + b + 1))
+= cbor_case_bound (cbor2_bound b)
+
+and cbor2_bound (b: nat) : Tot (cbor2 b -> nat) (decreases (b + b))
+= if b = 0 then empty_elim #nat else cbor1_bound (b - 1)
+
+noeq
+type cbor = {
+  b: nat;
+  obj: (obj: cbor1 b { cbor1_bound b obj == b });
+}
+
+let cbor_bound (x: cbor) : Tot nat = x.b
+
+(* Raw data items, disregarding ordering of map entries *)
+
+type raw_data_item : eqtype
 = | Simple: (v: simple_value) -> raw_data_item
   | Int64: (typ: major_type_uint64_or_neg_int64) -> (v: U64.t) -> raw_data_item
   | String: (typ: major_type_byte_string_or_text_string) -> (v: Seq.seq U8.t { FStar.UInt.fits (Seq.length v) U64.n }) -> raw_data_item // Section 3.1: "a string containing an invalid UTF-8 sequence is well-formed but invalid", so we don't care about UTF-8 specifics here.
